compilation.v : Lemmes + Definitions

compilation.v
@@ -1,9 +1,5 @@
-Load "Bureau/TER/CAM".
-Load "Bureau/TER/Lambda_calcul".
-
-(*Notation "lpush" := (push lambda_term).*)
-
-
+Load "CAM".
+Load "Lambda_Calcul".
 
 Fixpoint traduction (t : lambda_term) : option (code lambda_term) :=
 match t with
@@ -22,3 +18,24 @@ match t with
     end
 end.
 
+Notation "'constantel'" := (constante lambda_term).
+Notation "'pairel'" := (paire lambda_term).
+Notation "'quotel'" := (quote lambda_term).
+Notation "'consl'" := (cons lambda_term).
+Notation "'appl'" := (app lambda_term).
+Definition empty_stack := (constantel (var 0))::nil.
+
+Goal forall c1 c2 : code lambda_term, traduction (lapp id (var 1)) = Some c1 -> traduction (var 1) = Some c2 -> cam_reduction_ref_trans lambda_term empty_stack c1 empty_stack c2.
+Proof.
+intros.
+inversion H; inversion H0.
+apply reduc_trans with
+((constantel (var 0))::(constantel (var 0))::nil)
+((quotel (var 1)) :: consl :: (appl) :: nil).
+apply reduc_cas_base; remove_simple_cam_reduc.
+apply reduc_trans with
+((constantel (var 1)) :: (constantel (var 0))::nil)
+(consl :: appl :: nil).
+apply reduc_cas_base; remove_simple_cam_reduc.
+
+Lemma correction : forall (t t' : lambda_term) (c1 c2 : code lambda_term), t ->β t' -> traduction t = Some c1 -> traduction t' = Some c2 -> cam_reduction_ref_trans lambda_term empty_stack c1 empty_stack c2.
